Rename mlifytable_guarded to mlifyable_in

io/ho_examples/Callback.Example.fst
@@ -33,14 +33,14 @@ let cb_mlifyable : mlifyable cb =
     (fun fd h -> is_open fd h)
     (fun fd h _ lt -> lt == [])
 
-let cb_mlifyable_guarded : mlifyable_guarded_arr1 file_descr bool (fun fd h -> is_open fd h) (fun fd h r lt -> lt == []) pi = {
+let cb_mlifyable_in : mlifyable_in_arr1 file_descr bool (fun fd h -> is_open fd h) (fun fd h r lt -> lt == []) pi = {
   ca1 = importable_safe_importable file_descr;
   cmlifyable1 = cb_mlifyable;
   cpi1 = ()
 }
 
 private
-let lemma_c1post () : squash (forall (x:cb_mlifyable_guarded.cmlifyable1.matype) h lt. True /\ enforced_locally pi h lt ==> (exists (r:maybe unit). enforced_locally pi h lt)) by (explode (); witness (`(Inl ())))= ()
+let lemma_c1post () : squash (forall (x:cb_mlifyable_in.cmlifyable1.matype) h lt. True /\ enforced_locally pi h lt ==> (exists (r:maybe unit). enforced_locally pi h lt)) by (explode (); witness (`(Inl ())))= ()
 
 private
 let lemma_c2post () : squash (forall h lt. enforced_locally pi h lt  ==> enforced_locally pi h lt) =
@@ -55,7 +55,7 @@ let pp_post_monitorable : monitorable_hist (fun fd h -> True) (fun fd h r lt -> 
 let ctx_instrumentable : instrumentable ctx pi =
   instrumentable_HO_arr1_out_importable file_descr bool (fun fd h -> is_open fd h) (fun fd h r lt -> lt == []) unit (fun h -> True) (fun h r lt -> enforced_locally pi h lt) pi
   #(importable_safe_importable _ #(safe_importable_ml (maybe unit) #(mlfo_maybe unit #(ML_FO mlfo_unit))))
-  #cb_mlifyable_guarded
+  #cb_mlifyable_in
   #pp_post_monitorable
   
 let pp_mlifyable : mlifyable pp =
